# AP Calculus AB Unit 3: Differentiation - Composite, Implicit, and Inverse Functions Study Guides

:::GUIDE:::
unit::=Unit 3
title::=üìê Unit 3: Advanced Differentiation Complete Guide
desc::=Master the chain rule for differentiating composite functions - the most powerful differentiation technique
diff::=Hard
time::=50 minutes
tags::=chain rule, composite functions, derivatives
content::=

# ‚õìÔ∏è The Chain Rule

## üéØ What Is a Composite Function?

A function inside another function! ü™Ü

### Composition Notation

If $f(x) = x^2$ and $g(x) = 3x + 1$:

$$f(g(x)) = f(3x+1) = (3x+1)^2$$

The "inner" function is $g(x) = 3x+1$
The "outer" function is $f(u) = u^2$

---

## ‚õìÔ∏è The Chain Rule

### The Rule

If $y = f(g(x))$, then:

$$\frac{dy}{dx} = f'(g(x)) \cdot g'(x)$$

**"Derivative of outside times derivative of inside"**

### Leibniz Notation

If $y = f(u)$ and $u = g(x)$:

$$\frac{dy}{dx} = \frac{dy}{du} \cdot \frac{du}{dx}$$

The $du$'s "cancel" like fractions! ‚ú®

---

## üìä Chain Rule Process

### Step-by-Step

1. Identify the **outer function** (what happens last)
2. Identify the **inner function** (what's inside)
3. Differentiate the outer, keeping inner unchanged
4. Multiply by derivative of inner

### Visual Process

```
y = f(g(x))

Step 1: f'(g(x))     ‚Üê derivative of outer
Step 2: √ó g'(x)      ‚Üê times derivative of inner

Result: f'(g(x)) ¬∑ g'(x)
```

---

## üîß Basic Chain Rule Examples

### Example 1: $(3x+1)^5$

**Outer**: $u^5$
**Inner**: $3x+1$

$$\frac{d}{dx}[(3x+1)^5] = 5(3x+1)^4 \cdot 3 = 15(3x+1)^4$$

### Example 2: $\sqrt{x^2+1}$

Rewrite: $(x^2+1)^{1/2}$

**Outer**: $u^{1/2}$
**Inner**: $x^2+1$

$$= \frac{1}{2}(x^2+1)^{-1/2} \cdot 2x = \frac{x}{\sqrt{x^2+1}}$$

### Example 3: $(2x^3-5)^{-2}$

**Outer**: $u^{-2}$
**Inner**: $2x^3-5$

$$= -2(2x^3-5)^{-3} \cdot 6x^2 = \frac{-12x^2}{(2x^3-5)^3}$$

---

## üìê Chain Rule with Trig Functions

### Pattern

$$\frac{d}{dx}[\sin(u)] = \cos(u) \cdot u'$$

$$\frac{d}{dx}[\cos(u)] = -\sin(u) \cdot u'$$

### Examples

| Function | Derivative |
|----------|------------|
| $\sin(3x)$ | $\cos(3x) \cdot 3 = 3\cos(3x)$ |
| $\cos(x^2)$ | $-\sin(x^2) \cdot 2x = -2x\sin(x^2)$ |
| $\tan(5x)$ | $\sec^2(5x) \cdot 5 = 5\sec^2(5x)$ |
| $\sin^2(x)$ | $2\sin(x) \cdot \cos(x) = \sin(2x)$ |

### ‚ö†Ô∏è Watch Out!

| Expression | Meaning |
|------------|---------|
| $\sin^2(x)$ | $(\sin x)^2$ - outer is squaring |
| $\sin(x^2)$ | $\sin(x^2)$ - outer is sine |

---

## üìê Chain Rule with Exponentials

### Natural Exponential

$$\frac{d}{dx}[e^{u}] = e^{u} \cdot u'$$

### Examples

| Function | Derivative |
|----------|------------|
| $e^{3x}$ | $e^{3x} \cdot 3 = 3e^{3x}$ |
| $e^{x^2}$ | $e^{x^2} \cdot 2x = 2xe^{x^2}$ |
| $e^{-x}$ | $e^{-x} \cdot (-1) = -e^{-x}$ |
| $e^{\sin x}$ | $e^{\sin x} \cdot \cos x$ |

### General Exponential

$$\frac{d}{dx}[a^{u}] = a^{u} \ln(a) \cdot u'$$

---

## üìê Chain Rule with Logarithms

### Natural Log

$$\frac{d}{dx}[\ln(u)] = \frac{1}{u} \cdot u' = \frac{u'}{u}$$

### Examples

| Function | Derivative |
|----------|------------|
| $\ln(3x)$ | $\frac{3}{3x} = \frac{1}{x}$ |
| $\ln(x^2+1)$ | $\frac{2x}{x^2+1}$ |
| $\ln(\sin x)$ | $\frac{\cos x}{\sin x} = \cot x$ |
| $\ln(e^x)$ | $\frac{e^x}{e^x} = 1$ (or just = $x$) |

---

## üîó Multiple Chain Rule Applications

### Nested Functions

For $(outer(middle(inner)))$:

$$\frac{d}{dx} = outer' \cdot middle' \cdot inner'$$

### Example: $\sin^3(2x)$

This is $(\sin(2x))^3$

$$= 3(\sin(2x))^2 \cdot \cos(2x) \cdot 2$$
$$= 6\sin^2(2x)\cos(2x)$$

### Example: $e^{\cos(3x)}$

$$= e^{\cos(3x)} \cdot (-\sin(3x)) \cdot 3$$
$$= -3\sin(3x)e^{\cos(3x)}$$

---

## üìä Chain Rule Reference Table

| Form | Derivative |
|------|------------|
| $[u]^n$ | $n[u]^{n-1} \cdot u'$ |
| $\sin(u)$ | $\cos(u) \cdot u'$ |
| $\cos(u)$ | $-\sin(u) \cdot u'$ |
| $\tan(u)$ | $\sec^2(u) \cdot u'$ |
| $e^u$ | $e^u \cdot u'$ |
| $\ln(u)$ | $\frac{u'}{u}$ |
| $a^u$ | $a^u \ln(a) \cdot u'$ |

---

## üéØ AP Exam Tips

| Concept | Remember |
|---------|----------|
| Chain rule | Outer' √ó Inner' |
| Leibniz | $\frac{dy}{dx} = \frac{dy}{du} \cdot \frac{du}{dx}$ |
| Always | Don't forget the inner derivative! |
| Common error | Forgetting to multiply by $u'$ |

:::GUIDE:::
unit::=Unit 3
title::=Implicit Differentiation
desc::=Learn to find derivatives when y cannot be isolated - essential for curves and relations
diff::=Hard
time::=45 minutes
tags::=implicit differentiation, dy/dx, curves
content::=

# üîç Implicit Differentiation

## üìê Explicit vs. Implicit

### Explicit Functions

$y$ is solved in terms of $x$:

$$y = x^2 + 3x - 5$$
$$y = \sin(x) + e^x$$

### Implicit Relations

$x$ and $y$ are mixed together:

$$x^2 + y^2 = 25$$ (circle)
$$x^3 + y^3 = 6xy$$ (folium)
$$xy = 1$$ (hyperbola)

---

## üßÆ The Implicit Process

### Key Insight

When differentiating $y$ with respect to $x$:

$$\frac{d}{dx}[y] = \frac{dy}{dx}$$

This is just the chain rule where $y$ is a function of $x$!

### The Process

1. Differentiate **both sides** with respect to $x$
2. When differentiating a $y$ term, multiply by $\frac{dy}{dx}$
3. Collect all $\frac{dy}{dx}$ terms on one side
4. Factor out $\frac{dy}{dx}$
5. Solve for $\frac{dy}{dx}$

---

## üîß Basic Examples

### Example 1: Circle $x^2 + y^2 = 25$

Differentiate both sides:
$$\frac{d}{dx}[x^2] + \frac{d}{dx}[y^2] = \frac{d}{dx}[25]$$

$$2x + 2y\frac{dy}{dx} = 0$$

Solve for $\frac{dy}{dx}$:
$$2y\frac{dy}{dx} = -2x$$

$$\frac{dy}{dx} = -\frac{x}{y}$$

### Example 2: $xy = 1$

Use **product rule** on $xy$:
$$\frac{d}{dx}[xy] = \frac{d}{dx}[1]$$

$$x\frac{dy}{dx} + y \cdot 1 = 0$$

$$\frac{dy}{dx} = -\frac{y}{x}$$

### Example 3: $x^2 + xy + y^2 = 7$

$$2x + \left(x\frac{dy}{dx} + y\right) + 2y\frac{dy}{dx} = 0$$

Collect $\frac{dy}{dx}$ terms:
$$x\frac{dy}{dx} + 2y\frac{dy}{dx} = -2x - y$$

Factor:
$$\frac{dy}{dx}(x + 2y) = -2x - y$$

Solve:
$$\frac{dy}{dx} = \frac{-2x - y}{x + 2y}$$

---

## üìä Common Implicit Patterns

### Differentiating $y^n$

$$\frac{d}{dx}[y^n] = ny^{n-1} \cdot \frac{dy}{dx}$$

| Expression | Derivative |
|------------|------------|
| $y^2$ | $2y\frac{dy}{dx}$ |
| $y^3$ | $3y^2\frac{dy}{dx}$ |
| $\sqrt{y}$ | $\frac{1}{2\sqrt{y}}\frac{dy}{dx}$ |
| $\frac{1}{y}$ | $-\frac{1}{y^2}\frac{dy}{dx}$ |

### Products with $y$

Use product rule:

| Expression | Derivative |
|------------|------------|
| $xy$ | $x\frac{dy}{dx} + y$ |
| $x^2y$ | $x^2\frac{dy}{dx} + 2xy$ |
| $xy^2$ | $x \cdot 2y\frac{dy}{dx} + y^2$ |

### Trig with $y$

| Expression | Derivative |
|------------|------------|
| $\sin(y)$ | $\cos(y)\frac{dy}{dx}$ |
| $\cos(y)$ | $-\sin(y)\frac{dy}{dx}$ |
| $e^y$ | $e^y\frac{dy}{dx}$ |
| $\ln(y)$ | $\frac{1}{y}\frac{dy}{dx}$ |

---

## üîß Advanced Examples

### Example: $\sin(xy) = x$

Use chain rule on $\sin(xy)$:
$$\cos(xy) \cdot \frac{d}{dx}[xy] = 1$$

$$\cos(xy) \cdot \left(x\frac{dy}{dx} + y\right) = 1$$

$$x\cos(xy)\frac{dy}{dx} + y\cos(xy) = 1$$

$$\frac{dy}{dx} = \frac{1 - y\cos(xy)}{x\cos(xy)}$$

### Example: $e^{xy} = x + y$

$$e^{xy} \cdot \left(x\frac{dy}{dx} + y\right) = 1 + \frac{dy}{dx}$$

$$xe^{xy}\frac{dy}{dx} + ye^{xy} = 1 + \frac{dy}{dx}$$

$$xe^{xy}\frac{dy}{dx} - \frac{dy}{dx} = 1 - ye^{xy}$$

$$\frac{dy}{dx}(xe^{xy} - 1) = 1 - ye^{xy}$$

$$\frac{dy}{dx} = \frac{1 - ye^{xy}}{xe^{xy} - 1}$$

---

## üìà Finding Tangent Lines

### Process

1. Use implicit differentiation to find $\frac{dy}{dx}$
2. Plug in the point to find the slope
3. Use point-slope form

### Example

Find tangent to $x^2 + y^2 = 25$ at $(3, 4)$

**Step 1**: $\frac{dy}{dx} = -\frac{x}{y}$

**Step 2**: At $(3, 4)$: $m = -\frac{3}{4}$

**Step 3**: $y - 4 = -\frac{3}{4}(x - 3)$

**Answer**: $y = -\frac{3}{4}x + \frac{25}{4}$

---

## ‚ö†Ô∏è Common Mistakes

| Mistake | Correct |
|---------|---------|
| Forgetting $\frac{dy}{dx}$ on $y$ terms | Every $y$ term needs $\frac{dy}{dx}$ |
| Product rule errors | $xy \to x\frac{dy}{dx} + y$ |
| Not solving for $\frac{dy}{dx}$ | Isolate it! |
| Wrong chain rule | $y^2 \to 2y\frac{dy}{dx}$, not $2y$ |

---

## üéØ AP Exam Tips

| Concept | Remember |
|---------|----------|
| $\frac{d}{dx}[y] = \frac{dy}{dx}$ | Chain rule! |
| Process | Differentiate ‚Üí Collect ‚Üí Factor ‚Üí Solve |
| Products | Always use product rule with $xy$ |
| Tangent lines | Find slope, use point-slope form |

:::GUIDE:::
unit::=Unit 3
title::=Derivatives of Inverse Functions
desc::=Learn to differentiate inverse functions including inverse trigonometric functions
diff::=Hard
time::=45 minutes
tags::=inverse functions, arcsin, arccos, arctan, derivatives
content::=

# üîÑ Derivatives of Inverse Functions

## üîÑ Inverse Function Review

### What Is an Inverse?

If $f(x)$ takes $a$ to $b$, then $f^{-1}(x)$ takes $b$ back to $a$.

$$f(a) = b \iff f^{-1}(b) = a$$

### Graphical Relationship

The graph of $f^{-1}$ is the **reflection** of $f$ across $y = x$

```
    y
    ‚îÇ     /f(x)
    ‚îÇ    /
    ‚îÇ   /  y = x
    ‚îÇ  / /
    ‚îÇ / / 
    ‚îÇ//  f‚Åª¬π(x)
‚îÄ‚îÄ‚îÄ‚îÄ‚îº‚îÄ‚îÄ‚îÄ‚îÄ‚îÄ‚îÄ‚îÄ‚îÄ‚îÄ‚îÄ‚îÄ‚îÄ x
    ‚îÇ
```

---

## üìê Derivative of Inverse Function

### The Formula

If $f$ and $f^{-1}$ are inverses:

$$\left(f^{-1}\right)'(x) = \frac{1}{f'(f^{-1}(x))}$$

### Alternate Form

If $g = f^{-1}$, then:

$$g'(x) = \frac{1}{f'(g(x))}$$

### Why Does This Work?

Since $f(f^{-1}(x)) = x$:

Differentiate both sides (chain rule):
$$f'(f^{-1}(x)) \cdot (f^{-1})'(x) = 1$$

Solve:
$$(f^{-1})'(x) = \frac{1}{f'(f^{-1}(x))}$$

---

## üîß Examples

### Example 1

If $f(x) = x^3 + 1$, find $(f^{-1})'(9)$.

**Step 1**: Find where $f(x) = 9$
$$x^3 + 1 = 9 \implies x^3 = 8 \implies x = 2$$

So $f^{-1}(9) = 2$

**Step 2**: Find $f'(x)$
$$f'(x) = 3x^2$$

**Step 3**: Apply formula
$$(f^{-1})'(9) = \frac{1}{f'(f^{-1}(9))} = \frac{1}{f'(2)} = \frac{1}{3(2)^2} = \frac{1}{12}$$

### Example 2

Given: $f(4) = 7$ and $f'(4) = 3$

Find $(f^{-1})'(7)$

Since $f(4) = 7$, we have $f^{-1}(7) = 4$

$$(f^{-1})'(7) = \frac{1}{f'(f^{-1}(7))} = \frac{1}{f'(4)} = \frac{1}{3}$$

---

## üìê Inverse Trig Derivatives

### The Six Inverse Trig Functions

| Function | Notation | Domain |
|----------|----------|--------|
| Inverse sine | $\arcsin x$ or $\sin^{-1}x$ | $[-1, 1]$ |
| Inverse cosine | $\arccos x$ or $\cos^{-1}x$ | $[-1, 1]$ |
| Inverse tangent | $\arctan x$ or $\tan^{-1}x$ | All reals |

---

## üìä Inverse Trig Derivative Formulas

### The Big Three (AP Calc AB)

$$\frac{d}{dx}[\arcsin x] = \frac{1}{\sqrt{1-x^2}}$$

$$\frac{d}{dx}[\arccos x] = -\frac{1}{\sqrt{1-x^2}}$$

$$\frac{d}{dx}[\arctan x] = \frac{1}{1+x^2}$$

### Memory Aid

| Function | Derivative | Note |
|----------|------------|------|
| $\arcsin x$ | $\frac{1}{\sqrt{1-x^2}}$ | Square root |
| $\arccos x$ | $-\frac{1}{\sqrt{1-x^2}}$ | Negative of arcsin |
| $\arctan x$ | $\frac{1}{1+x^2}$ | No square root |

---

## üßÆ Deriving Arcsin Derivative

### Proof

Let $y = \arcsin x$, so $\sin y = x$

Differentiate implicitly:
$$\cos y \cdot \frac{dy}{dx} = 1$$

$$\frac{dy}{dx} = \frac{1}{\cos y}$$

Since $\sin^2 y + \cos^2 y = 1$:
$$\cos y = \sqrt{1 - \sin^2 y} = \sqrt{1 - x^2}$$

Therefore:
$$\frac{d}{dx}[\arcsin x] = \frac{1}{\sqrt{1-x^2}}$$

---

## üîß Chain Rule with Inverse Trig

### General Forms

$$\frac{d}{dx}[\arcsin(u)] = \frac{u'}{\sqrt{1-u^2}}$$

$$\frac{d}{dx}[\arccos(u)] = -\frac{u'}{\sqrt{1-u^2}}$$

$$\frac{d}{dx}[\arctan(u)] = \frac{u'}{1+u^2}$$

### Examples

| Function | Derivative |
|----------|------------|
| $\arcsin(2x)$ | $\frac{2}{\sqrt{1-4x^2}}$ |
| $\arctan(x^2)$ | $\frac{2x}{1+x^4}$ |
| $\arccos(e^x)$ | $-\frac{e^x}{\sqrt{1-e^{2x}}}$ |
| $\arcsin(\sqrt{x})$ | $\frac{1/(2\sqrt{x})}{\sqrt{1-x}} = \frac{1}{2\sqrt{x-x^2}}$ |

---

## üìä Complete Inverse Trig Table

| Function | Derivative |
|----------|------------|
| $\arcsin x$ | $\frac{1}{\sqrt{1-x^2}}$ |
| $\arccos x$ | $-\frac{1}{\sqrt{1-x^2}}$ |
| $\arctan x$ | $\frac{1}{1+x^2}$ |
| $\text{arccot } x$ | $-\frac{1}{1+x^2}$ |
| $\text{arcsec } x$ | $\frac{1}{|x|\sqrt{x^2-1}}$ |
| $\text{arccsc } x$ | $-\frac{1}{|x|\sqrt{x^2-1}}$ |

*Note: Only arcsin, arccos, arctan typically on AP Calc AB*

---

## ‚ö†Ô∏è Common Mistakes

| Mistake | Correct |
|---------|---------|
| Confusing $\sin^{-1}x$ with $\frac{1}{\sin x}$ | $\sin^{-1}x = \arcsin x$ |
| Wrong signs | $\arccos$ has negative derivative |
| Forgetting chain rule | $\arcsin(2x)$ needs $√ó 2$ |
| Domain issues | $\arcsin x$ only for $|x| \leq 1$ |

---

## üéØ AP Exam Tips

| Function | Derivative |
|----------|------------|
| $\arcsin u$ | $\frac{u'}{\sqrt{1-u^2}}$ |
| $\arccos u$ | $-\frac{u'}{\sqrt{1-u^2}}$ |
| $\arctan u$ | $\frac{u'}{1+u^2}$ |
| Inverse function | $\frac{1}{f'(f^{-1}(x))}$ |

:::GUIDE:::
unit::=Unit 3
title::=Higher-Order Derivatives and Selecting Procedures
desc::=Learn about second and higher derivatives and how to choose the right differentiation technique
diff::=Medium
time::=35 minutes
tags::=second derivative, higher order, procedures
content::=

# üìà Higher-Order Derivatives

## üìä Second Derivatives

### Definition

The derivative of the derivative!

$$f''(x) = \frac{d}{dx}[f'(x)]$$

### Notations

| Notation | Read As |
|----------|---------|
| $f''(x)$ | "f double prime" |
| $y''$ | "y double prime" |
| $\frac{d^2y}{dx^2}$ | "d two y dx squared" |
| $\frac{d^2}{dx^2}[f]$ | "second derivative of f" |

---

## üîß Finding Second Derivatives

### Example 1

$f(x) = x^4 - 3x^2 + 5x$

$f'(x) = 4x^3 - 6x + 5$

$f''(x) = 12x^2 - 6$

### Example 2

$y = \sin(2x)$

$y' = 2\cos(2x)$

$y'' = 2 \cdot (-\sin(2x)) \cdot 2 = -4\sin(2x)$

### Example 3

$f(x) = e^{3x}$

$f'(x) = 3e^{3x}$

$f''(x) = 9e^{3x}$

---

## üìê Higher Order Derivatives

### Third, Fourth, and Beyond

| Order | Notation |
|-------|----------|
| Third | $f'''(x)$ or $f^{(3)}(x)$ |
| Fourth | $f^{(4)}(x)$ |
| nth | $f^{(n)}(x)$ |

### Example: $f(x) = x^5$

| Derivative | Result |
|------------|--------|
| $f'(x)$ | $5x^4$ |
| $f''(x)$ | $20x^3$ |
| $f'''(x)$ | $60x^2$ |
| $f^{(4)}(x)$ | $120x$ |
| $f^{(5)}(x)$ | $120$ |
| $f^{(6)}(x)$ | $0$ |

---

## üîÑ Pattern Recognition

### For $f(x) = e^{ax}$

All derivatives have pattern:
$$f^{(n)}(x) = a^n e^{ax}$$

### For $f(x) = \sin x$

| n | $f^{(n)}(x)$ |
|---|--------------|
| 1 | $\cos x$ |
| 2 | $-\sin x$ |
| 3 | $-\cos x$ |
| 4 | $\sin x$ |
| 5 | $\cos x$ |

Repeats every 4! So:
$$f^{(100)}(x) = \sin x$$ (since $100 \div 4 = 25$ remainder 0)

---

## üìä Implicit Second Derivatives

### Process

1. Find $\frac{dy}{dx}$ using implicit differentiation
2. Differentiate again, treating $y$ as function of $x$
3. Substitute $\frac{dy}{dx}$ from step 1

### Example: $x^2 + y^2 = 25$

**Step 1**: Find $\frac{dy}{dx}$
$$2x + 2y\frac{dy}{dx} = 0$$
$$\frac{dy}{dx} = -\frac{x}{y}$$

**Step 2**: Differentiate $\frac{dy}{dx} = -\frac{x}{y}$
$$\frac{d^2y}{dx^2} = -\frac{y \cdot 1 - x \cdot \frac{dy}{dx}}{y^2}$$

**Step 3**: Substitute $\frac{dy}{dx} = -\frac{x}{y}$
$$= -\frac{y - x \cdot (-\frac{x}{y})}{y^2} = -\frac{y + \frac{x^2}{y}}{y^2}$$
$$= -\frac{\frac{y^2 + x^2}{y}}{y^2} = -\frac{y^2 + x^2}{y^3}$$

Since $x^2 + y^2 = 25$:
$$\frac{d^2y}{dx^2} = -\frac{25}{y^3}$$

---

## üéØ Selecting Differentiation Procedures

### Decision Flowchart

```
Is y explicit (solved for y)?
‚îú‚îÄ YES: Use basic rules
‚îî‚îÄ NO: Use implicit differentiation

Is it a composite function?
‚îú‚îÄ YES: Use chain rule
‚îî‚îÄ NO: Check for products/quotients

Is it a product of functions?
‚îú‚îÄ YES: Use product rule
‚îî‚îÄ NO: Continue

Is it a quotient of functions?
‚îú‚îÄ YES: Use quotient rule
‚îî‚îÄ NO: Use basic rules
```

### Quick Reference

| Situation | Rule to Use |
|-----------|-------------|
| $f(g(x))$ | Chain rule |
| $f \cdot g$ | Product rule |
| $\frac{f}{g}$ | Quotient rule |
| $x$ and $y$ mixed | Implicit |
| $f^{-1}$ | Inverse function rule |
| $\arcsin, \arctan$ | Inverse trig formulas |

---

## üîß Combined Examples

### Example 1: Multiple Rules

Find $\frac{d}{dx}[x^2 \sin(3x)]$

**Rules needed**: Product + Chain

$$= x^2 \cdot \cos(3x) \cdot 3 + \sin(3x) \cdot 2x$$
$$= 3x^2\cos(3x) + 2x\sin(3x)$$

### Example 2: Quotient + Chain

Find $\frac{d}{dx}\left[\frac{e^{2x}}{x+1}\right]$

$$= \frac{(x+1) \cdot 2e^{2x} - e^{2x} \cdot 1}{(x+1)^2}$$
$$= \frac{e^{2x}(2x+2-1)}{(x+1)^2} = \frac{e^{2x}(2x+1)}{(x+1)^2}$$

### Example 3: Implicit + Chain

$\sin(xy) = y$

$$\cos(xy) \cdot \left(y + x\frac{dy}{dx}\right) = \frac{dy}{dx}$$
$$y\cos(xy) + x\cos(xy)\frac{dy}{dx} = \frac{dy}{dx}$$
$$y\cos(xy) = \frac{dy}{dx} - x\cos(xy)\frac{dy}{dx}$$
$$y\cos(xy) = \frac{dy}{dx}(1 - x\cos(xy))$$
$$\frac{dy}{dx} = \frac{y\cos(xy)}{1 - x\cos(xy)}$$

---

## üéØ AP Exam Tips

| Concept | Remember |
|---------|----------|
| Second derivative | Derivative of the derivative |
| Sin/Cos pattern | Repeats every 4 derivatives |
| $e^{ax}$ pattern | $f^{(n)} = a^n e^{ax}$ |
| Procedure selection | Identify structure first |

:::GUIDE:::
unit::=Unit 3
title::=Unit 3 AP Exam Strategies
desc::=Master key concepts and problem-solving strategies for Unit 3 of the AP Calculus AB exam
diff::=Medium
time::=30 minutes
tags::=AP exam, strategies, Unit 3
content::=

# üìù Unit 3 AP Exam Strategies

## üìä Unit Weight

| Exam Section | Unit 3 Weight |
|--------------|---------------|
| Multiple Choice | ~9-13% |
| Free Response | Very common |

---

## üîë Must-Know Formulas

### Chain Rule

$$\frac{d}{dx}[f(g(x))] = f'(g(x)) \cdot g'(x)$$

### Common Chain Rule Forms

| Form | Derivative |
|------|------------|
| $(u)^n$ | $n(u)^{n-1} \cdot u'$ |
| $\sin(u)$ | $\cos(u) \cdot u'$ |
| $\cos(u)$ | $-\sin(u) \cdot u'$ |
| $e^u$ | $e^u \cdot u'$ |
| $\ln(u)$ | $\frac{u'}{u}$ |

### Implicit Differentiation

When differentiating $y$: multiply by $\frac{dy}{dx}$

### Inverse Function

$$(f^{-1})'(x) = \frac{1}{f'(f^{-1}(x))}$$

### Inverse Trig

| Function | Derivative |
|----------|------------|
| $\arcsin u$ | $\frac{u'}{\sqrt{1-u^2}}$ |
| $\arccos u$ | $-\frac{u'}{\sqrt{1-u^2}}$ |
| $\arctan u$ | $\frac{u'}{1+u^2}$ |

---

## ‚úçÔ∏è Sample MC Questions

### Question 1

Find $\frac{d}{dx}[(2x+1)^4]$

(A) $4(2x+1)^3$
(B) $8(2x+1)^3$
(C) $(2x+1)^3$
(D) $4(2x+1)^4$

**Solution**: Chain rule
$$= 4(2x+1)^3 \cdot 2 = 8(2x+1)^3$$

**Answer: (B)**

### Question 2

If $x^2 + y^2 = 16$, find $\frac{dy}{dx}$

(A) $\frac{x}{y}$
(B) $-\frac{x}{y}$
(C) $-\frac{y}{x}$
(D) $\frac{2x}{2y}$

**Solution**: Implicit differentiation
$$2x + 2y\frac{dy}{dx} = 0$$
$$\frac{dy}{dx} = -\frac{x}{y}$$

**Answer: (B)**

### Question 3

Find $\frac{d}{dx}[\arctan(3x)]$

(A) $\frac{3}{1+9x^2}$
(B) $\frac{1}{1+9x^2}$
(C) $\frac{3}{1+3x^2}$
(D) $\frac{1}{\sqrt{1-9x^2}}$

**Solution**: 
$$= \frac{3}{1+(3x)^2} = \frac{3}{1+9x^2}$$

**Answer: (A)**

### Question 4

If $f(5) = 2$ and $f'(5) = 7$, find $(f^{-1})'(2)$

(A) $\frac{1}{7}$
(B) $7$
(C) $\frac{1}{2}$
(D) $\frac{2}{7}$

**Solution**: Since $f(5) = 2$, we have $f^{-1}(2) = 5$

$$(f^{-1})'(2) = \frac{1}{f'(f^{-1}(2))} = \frac{1}{f'(5)} = \frac{1}{7}$$

**Answer: (A)**

---

## ‚úçÔ∏è Sample FR Question

**Question**: Let $f(x) = \sin(x^2)$

(a) Find $f'(x)$.

(b) Find $f''(x)$.

(c) Find the equation of the tangent line to $y = f(x)$ at $x = \sqrt{\pi}$.

**Solution**:

(a) Using chain rule:
$$f'(x) = \cos(x^2) \cdot 2x = 2x\cos(x^2)$$

(b) Using product rule and chain rule:
$$f''(x) = 2\cos(x^2) + 2x \cdot (-\sin(x^2)) \cdot 2x$$
$$= 2\cos(x^2) - 4x^2\sin(x^2)$$

(c) At $x = \sqrt{\pi}$:
- $f(\sqrt{\pi}) = \sin(\pi) = 0$
- $f'(\sqrt{\pi}) = 2\sqrt{\pi}\cos(\pi) = 2\sqrt{\pi}(-1) = -2\sqrt{\pi}$

Tangent line:
$$y - 0 = -2\sqrt{\pi}(x - \sqrt{\pi})$$
$$y = -2\sqrt{\pi}x + 2\pi$$

---

## ‚ö†Ô∏è Common Mistakes

### Chain Rule Errors

| Mistake | Correct |
|---------|---------|
| Forgetting inner derivative | Always multiply by $u'$ |
| $(3x)^2 \to 6x$ | $(3x)^2 \to 2(3x) \cdot 3 = 18x$ |

### Implicit Differentiation Errors

| Mistake | Correct |
|---------|---------|
| Forgetting $\frac{dy}{dx}$ on $y$ terms | Every $y$ needs it |
| Not collecting $\frac{dy}{dx}$ terms | Factor it out |

### Inverse Function Errors

| Mistake | Correct |
|---------|---------|
| Wrong formula direction | $(f^{-1})'(b) = \frac{1}{f'(a)}$ where $f(a) = b$ |
| Confusing $f^{-1}$ with $\frac{1}{f}$ | They're different! |

---

## üìã Unit 3 Checklist

### Before the Exam

‚úÖ Can apply chain rule with polynomials
‚úÖ Can apply chain rule with trig functions
‚úÖ Can apply chain rule with exponentials and logs
‚úÖ Can do implicit differentiation
‚úÖ Can find tangent lines for implicit curves
‚úÖ Know inverse function derivative formula
‚úÖ Know derivatives of arcsin, arccos, arctan
‚úÖ Can find second derivatives
‚úÖ Can recognize patterns in higher derivatives

---

## üîó Connections

### Unit 3 ‚Üí Unit 4

| Unit 3 | Application in Unit 4 |
|--------|----------------------|
| Implicit differentiation | Related rates |
| Chain rule | Related rates |
| All differentiation | Contextual problems |

### Unit 3 ‚Üí Unit 5

| Unit 3 | Application in Unit 5 |
|--------|----------------------|
| Second derivative | Concavity |
| $f''(x)$ | Inflection points |
| Differentiation | Optimization |

**Good luck! üçÄ**
